newest version

src/certificateGen.ml
@@ -7,15 +7,23 @@ let ps s = Feedback.msg_info (Pp.str s)
 
 let func_inv = Smartlocate.global_constant_with_alias (Libnames.qualid_of_string "RefineInv.FUNC")
 let eval_term = Smartlocate.global_constant_with_alias (Libnames.qualid_of_string "RefineInv.EVAL")
-let empty_sem_env = Smartlocate.global_constant_with_alias (Libnames.qualid_of_string "empty_sem_env")
+let empty_sem_env = Smartlocate.global_constant_with_alias (Libnames.qualid_of_string "SemanticsAux.empty_sem_env")
 let empty_namespace =
   Smartlocate.global_constant_with_alias (Libnames.qualid_of_string "CakeSem.Namespace.nsEmpty")
+
+let init_state_fun =
+  Smartlocate.global_constant_with_alias (Libnames.qualid_of_string "EvaluateDecsWrapper.init_st")
+
+let init_state = mkApp (mkConst init_state_fun, [|TypeGen.nat_type; TermGen.get_nat_constr "O" |])
 
 let extend_dec_env =
   Smartlocate.global_constant_with_alias (Libnames.qualid_of_string "CakeSem.SemanticsAux.extend_dec_env")
 
+let eval_decs_wrapper =
+  Smartlocate.global_constant_with_alias (Libnames.qualid_of_string "EvaluateDecsWrapper.eval_decs_wrapper")
+
 let mk_extend_dec_env new_env sem_env =
-  mkApp(mkConst extend_dec_env,[|TypeGen.val_type (); new_env; sem_env|])
+  mkApp (mkConst extend_dec_env,[|TypeGen.val_type; new_env; sem_env|])
 
 let mk_empty_namespace mType nType vType = mkApp(mkConst empty_namespace,[|mType; nType; vType|])
 
@@ -26,10 +34,26 @@ let add_constructor_to_sem_env name cake_constructor sem_env =
 
 let mkFUNC typ1 typ2 inv1 inv2 = mkApp(mkConst func_inv,[|typ1; typ2; inv1; inv2|])
 let mkEVAL cake_env exp inv = mkApp(mkConst eval_term,[|cake_env; exp; inv|])
-let mkEmptyEnv = mkApp(mkConst empty_sem_env,[|TypeGen.val_type ()|])
+let mk_empty_sem_env = mkApp(mkConst empty_sem_env,[|TypeGen.val_type|])
+
+let coq_fst sigma pair =
+  let hd, args = destApp sigma pair in
+  args.(2)
+
+let coq_snd sigma pair =
+  let hd, args = destApp sigma pair in
+  args.(3)
 
 (* sem_env val*)
-let current_cake_env = ref mkEmptyEnv
+let current_cake_env = ref mk_empty_sem_env
+let reset_current_cake_env () = current_cake_env := mk_empty_sem_env
+let current_cake_st = ref init_state
+let reset_current_cake_st () = current_cake_st := init_state
+let clear_semantic_environment () = reset_current_cake_env (); reset_current_cake_st ()
+
+let eval_dec decs env =
+  let eval_decs_wrapper = Smartlocate.global_constant_with_alias (Libnames.qualid_of_string "EvaluateDecsWrapper.eval_decs_wrapper") in
+  mkApp (mkConst eval_decs_wrapper, [| init_state; env; TermGen.list_to_coq_list decs TypeGen.dec_type |])
 
 (* Convert Debruijn numbers to named variables when applicable *)
 let rec rels_to_vars env typ =
@@ -59,11 +83,15 @@ let rec invariant_from_type env typ =
     fun id -> Nameops.add_suffix id "_INV" |> mkVar
 
   | Ind (name,univ) ->
-    Indmap.find name !InvGen.global_invariant_table
+    begin
+      try Indmap.find name !InvGen.global_invariant_table with
+      | Not_found -> (print_string "Invariant undefined"; raise Not_found)
+    end
 
   | Prod (name,typ',body) ->
     let env' = push_rel (LocalAssum (name,typ')) env in
     let body_inv = invariant_from_type env' body in
+    let sigma' = Evd.from_env env' in
 
     if isArity sigma typ' then
       let inv_id = String.concat "" [TermGen.name_to_str ~anon:"ANON" name.binder_name; "_INV"] |>
@@ -71,10 +99,10 @@ let rec invariant_from_type env typ =
       let inv_name = Name inv_id in
 
       let inv_type = mkProd(Context.annotR Name.Anonymous,mkRel 1,
-                            mkProd(Context.annotR Name.Anonymous,TypeGen.val_type (),mkProp)) in
-      let body_inv' = Vars.subst_var (InvGen.id_of_name ~anon:"ANON" name.binder_name) body_inv in
+                            mkProd(Context.annotR Name.Anonymous,TypeGen.val_type,mkProp)) in
+      let body_inv' = Vars.subst_var sigma' (InvGen.id_of_name ~anon:"ANON" name.binder_name) body_inv in
       let body_inv'' = Vars.lift 1 body_inv' in
-      let body_inv''' = Vars.subst_var inv_id body_inv'' in
+      let body_inv''' = Vars.subst_var sigma' inv_id body_inv'' in
 
       mkProd (name, typ', mkProd (Context.annotR inv_name, inv_type, body_inv'''))
     else
@@ -108,36 +136,89 @@ let create_certificate_theorem env cake_env term =
   let inv = invariant_from_type env typ in
   let exp = translate_term env term in
   let prods,decl = decompose_prod sigma inv in
-  (* working here *)
   let rels = Array.init (List.length prods / 2) (fun x -> mkRel ((x + 1) * 2))
              |> Array.to_list |> List.rev |> Array.of_list in
   let decl' = mkApp (decl, [|mkApp (term, rels)|]) in
   let prods' = List.map (fun (x,y) -> Context.Rel.Declaration.LocalAssum (x,y)) prods in
   it_mkProd_or_LetIn (mkEVAL cake_env exp decl') prods'
 
-let generate_certificate_theorem ref =
-    let glob_ref = locate_global_ref ref in
-    let global_env = Global.env () in
-    let sigma = Evd.from_env global_env in
+(* Definition DECL (st : state ST) (env : sem_env val) (decs : list dec) (st' : state ST) (env' : sem_env val) *)
+let create_decl_certificate_theorem start_st start_env =
+  let decl_constant = mkConst (Smartlocate.global_constant_with_alias (Libnames.qualid_of_string "DECL")) in
+  let rev_constant = mkConst (Smartlocate.global_constant_with_alias (Libnames.qualid_of_string "rev")) in
+  mkApp (decl_constant,
+         [| start_st; start_env;
+            mkApp (rev_constant, [| TypeGen.dec_type; !current_program |]);
+            !current_cake_st; !current_cake_env |])
+
+let generate_invariant_and_update_environment ref =
+  let glob_ref = locate_global_ref ref in
+  let global_env = Global.env () in
+  let sigma = Evd.from_env global_env in
+  match glob_ref with
+  | IndRef (name,_) | ConstructRef ((name,_),_) ->
+    InvGen.generate_refinement_invariant ref;
+    let cake_dec = translate_declaration ref in
+    let _ = add_dec_to_current_program cake_dec in
+    let eval_dec_term = eval_dec [cake_dec] !current_cake_env in
+    let res = Reductionops.nf_all global_env sigma eval_dec_term in
+    current_cake_env := Reductionops.nf_all global_env sigma (mk_extend_dec_env (coq_snd sigma res) !current_cake_env);
+    (* PrintDebug.print_econstr !current_cake_env; *)
+    current_cake_st := (coq_fst sigma res)
+
+  | _ -> raise (UnsupportedFeature "must be a reference to constructor or inductive type")
+
+let generate_certificate_theorem ~pm ~ref =
+  let glob_ref = locate_global_ref ref in
+  let global_env = Global.env () in
+  let sigma = Evd.from_env global_env in
+  let cake_dec = translate_declaration ref in
+  let eval_dec_term = eval_dec [cake_dec] !current_cake_env in
+    let res = Reductionops.nf_all global_env sigma eval_dec_term in
+    let old_cake_env = !current_cake_env in
+    let extended_env = mk_extend_dec_env (coq_snd sigma res) !current_cake_env in
+    (* PrintDebug.print_econstr extended_env; *)
+    let _ = add_dec_to_current_program cake_dec in
+    current_cake_env := Reductionops.nf_all global_env sigma extended_env;
     match glob_ref with
     | ConstRef const_name ->
       let x = Environ.lookup_constant const_name global_env in
       let certificate = begin
         match x.const_body with
         | Def const ->
-          create_certificate_theorem global_env !current_cake_env (EConstr.of_constr const)
+          create_certificate_theorem global_env old_cake_env (EConstr.of_constr const);
         | Undef _ -> raise (UnsupportedFeature "Axioms not supported")
         | _ -> raise (UnsupportedFeature "not doing this part right now")
       end in
-      let certificate_theorem_name = const_name |> Names.Constant.label |> Names.Label.to_id
-                                     |> Nameops.add_prefix "cake_" |> fun x -> Nameops.add_suffix x "_certificate_thm" in
+      let certificate_theorem_name =
+        const_name |> Names.Constant.label |> Names.Label.to_id
+        |> Nameops.add_prefix "cake_" |> fun x -> Nameops.add_suffix x "_certificate_thm" in
       let sigma', declaration_type = Typing.type_of ~refresh:true global_env sigma certificate in
-      let _ = Declare.declare_definition
-        ~info:(Declare.Info.make ())
-        ~cinfo:(Declare.CInfo.make ~name:certificate_theorem_name ~typ:(Some declaration_type) ())
-        ~opaque:false
-        ~body:certificate
-        sigma'
-      in
-      PrintDebug.print_econstr certificate
-    | _ -> ()
+
+      let open Declare in
+      let pm = OblState.empty in
+      (* let sigma'', evar =  Evarutil.new_evar global_env sigma' certificate in *)
+      (* let cinfo = CInfo.make ~name:certificate_theorem_name ~typ:(EConstr.to_constr sigma'' certificate) () in *)
+      let cinfo' = CInfo.make ~name:certificate_theorem_name ~typ:certificate () in
+      let info = Info.make () in
+      (* let obls_info,_,term,_ = RetrieveObl.retrieve_obligations global_env certificate_theorem_name sigma'' 0 evar certificate in *)
+      (* let pm,prog = Obls.add_definition ~pm ~cinfo ~term ~info ~uctx:(Evd.evar_universe_context sigma'') ~opaque:false obls_info in *)
+      pm, Declare.Proof.start ~info ~cinfo:cinfo' sigma'
+
+    (* | IndRef (mut_name,_) | ConstructRef ((mut_name,_),_) -> *)
+    | _ -> raise (UnsupportedFeature "need to come back here")
+
+let generate_decl_certificate_theorem ~pm prog_name =
+  let global_env = Global.env () in
+  let sigma = Evd.from_env global_env in
+
+  let certificate = create_decl_certificate_theorem init_state (mkApp (mkConst empty_sem_env, [| TypeGen.val_type |])) in
+  let certificate_theorem_name = Nameops.add_prefix "cake_prog_" (Nameops.add_suffix (Names.Id.of_string prog_name) "_certificate_thm") in
+
+  let sigma', declaration_type = Typing.type_of ~refresh:true global_env sigma certificate in
+
+  let open Declare in
+  let pm = OblState.empty in
+  let cinfo' = CInfo.make ~name:certificate_theorem_name ~typ:certificate () in
+  let info = Info.make () in
+  pm, Declare.Proof.start ~info ~cinfo:cinfo' sigma'
