theories/RefineInv.v
@@ -17,93 +17,8 @@ Definition ST := nat.
 (* environment manipulation *)
 Definition bind_variable_name name v (env : sem_env val) := update_sev env (nsBind name v (sev env)).
 
-(* Certificate theorem for CakeML expressions *)
-
-Definition EVAL (env : sem_env val) (e : exp) (inv : val -> Prop) :=
- forall st, exists v f st', evaluate [e] f st env = (st', Rval [v]) /\ inv v.
-
-Definition eval_rel (st : state ST) (env : sem_env val) (e : exp) (st' : state ST) (v : val) : Prop :=
-  exists (f : nat), evaluate [e] f st env = (st', Rval [v]).
-
-Definition app_returns (P Q : val -> Prop) (cl : val) :=
-  forall (v : val), P v ->
-               forall (st : state ST), exists env exp st' u,
-                 do_opapp [cl;v] = Some (env,exp) /\
-                   eval_rel st env exp st' u /\
-                   Q u.
-
-Definition FUNC {A B : Type} (AINV : A -> val -> Prop) (BINV : B -> val -> Prop) (f : A -> B) (cl : val) :=
-  forall x v, AINV x v -> exists u, BINV (f x) u /\ app_returns (AINV x) (BINV (f x)) cl.
-
-Theorem EVAL_EFun {A B : Type} (env : sem_env val) (AINV : A -> val -> Prop) (BINV : B -> val -> Prop) (f : A -> B) (n : varN) (body : exp) :
-  (forall (x : A) (v : val), AINV x v -> EVAL (bind_variable_name n v env) body (BINV (f x))) ->
-  EVAL env (EFun n body) ((FUNC AINV BINV f)).
-Proof.
-  unfold FUNC, EVAL, evaluate, app_returns, eval_rel.
-  intros H_body st.
-  do 3 eexists.
-  split; try (simp eval_or_match; reflexivity).
-  intros x v H_AINV_x_v.
-  destruct (H_body x v H_AINV_x_v st) as [v' [f' [st' [eval_body H_BINV_fx_v']]]].
-  eexists.
-  split; try apply H_BINV_fx_v'.
-  intros v0 H_AINV_x_v0 st0.
-  destruct (H_body x v0 H_AINV_x_v0 st0) as [v'' [f'' [st'' [eval_body' H_BINV_fx_v'']]]].
-  eexists.
-  exists body.
-  exists st''.
-  exists v''.
-  split; try reflexivity.
-  split; try apply H_BINV_fx_v''.
-  exists f''.
-  unfold evaluate.
-  assumption.
-  Unshelve.
-  constructor.
-Qed.
-
-Theorem EVAL_ELetrec_general : forall funs env exp P,
-  NoDup (map (fun '(x,y,z) => x) funs) ->
-  EVAL (update_sev env (build_rec_env funs env (sev env))) exp P ->
-  EVAL env (ELetrec funs exp) P.
-Proof.
-  unfold EVAL, evaluate.
-  intros funs env exp P HNoDup Hexp st.
-  specialize (Hexp st).
-  destruct Hexp as [v [f [st' [Hexp Hinv]]]].
-  exists v. exists f. exists st'.
-  split; try assumption.
-  - simp eval_or_match.
-    break_match; try assumption; try contradiction.
-Qed.
-
-(* EQ restricts an invariant to talk about a specific term *)
-Definition EQ {A : Type} (AINV : A -> val -> Prop) (a : A) := fun a' v => (a = a') /\ AINV a' v.
-
-Theorem EVAL_EQ {A : Type} : forall (AINV : A -> val -> Prop) (a : A) (e : exp) (env : sem_env val),
-  EVAL env e (AINV a) -> EVAL env e ((EQ AINV a) a).
-Proof.
-  unfold EVAL.
-  unfold EQ.
-  intros AINV a e env H st.
-  specialize (H st).
-  destruct H as [v [f [st' [Heval Hinv]]]].
-  exists v. exists f. exists st'.
-  auto.
-Qed.
-
-Theorem exists_EQ_INV_iff_INV : forall (A : Type) (AINV : A -> val -> Prop) a v, (exists a', EQ AINV a' a v) <-> AINV a v.
-Proof.
-  unfold EQ.
-  intros A AINV a v.
-  split; intro H.
-  destruct H as [a' [Ha'eqa HAINVa]].
-  auto.
-  exists a.
-  split; auto.
-Qed.
-
-Theorem use_maximum_fuel : forall fuels es fuel st env st' vs,
+(* fuel manipulation *)
+Theorem use_maximum_fuel : forall fuel fuels es st env st' vs,
     fuel <= list_max fuels ->
     eval_or_match true es fuel st env uu uu = (st', Rval vs) ->
     eval_or_match true es (list_max fuels) st env uu uu = (st', Rval vs).
@@ -168,6 +83,176 @@ Proof.
     assumption.
 Qed.
 
+(* Certificate theorem for CakeML expressions *)
+Definition EVAL (env : sem_env val) (e : exp) (inv : val -> Prop) :=
+ forall st, exists v f st', evaluate [e] f st env = (st', Rval [v]) /\ inv v.
+
+Definition eval_rel (st : state ST) (env : sem_env val) (e : exp) (st' : state ST) (v : val) : Prop :=
+  exists (f : nat), evaluate [e] f st env = (st', Rval [v]).
+
+Definition app_returns (P Q : val -> Prop) (cl : val) :=
+  forall (v : val), P v ->
+               forall (st : state ST), exists env exp st' u,
+                 do_opapp [cl;v] = Some (env,exp) /\
+                   eval_rel st env exp st' u /\
+                   Q u.
+
+Definition FUNC {A B : Type} (AINV : A -> val -> Prop) (BINV : B -> val -> Prop) (f : A -> B) (cl : val) :=
+  forall x v, AINV x v -> exists u, BINV (f x) u /\ app_returns (AINV x) (BINV (f x)) cl.
+
+Theorem EVAL_EFun {A B : Type} (env : sem_env val) (AINV : A -> val -> Prop) (BINV : B -> val -> Prop) (f : A -> B) (n : varN) (body : exp) :
+  (forall (x : A) (v : val), AINV x v -> EVAL (bind_variable_name n v env) body (BINV (f x))) ->
+  EVAL env (EFun n body) ((FUNC AINV BINV f)).
+Proof.
+  unfold FUNC, EVAL, evaluate, app_returns, eval_rel.
+  intros H_body st.
+  do 3 eexists.
+  split; try (simp eval_or_match; reflexivity).
+  intros x v H_AINV_x_v.
+  destruct (H_body x v H_AINV_x_v st) as [v' [f' [st' [eval_body H_BINV_fx_v']]]].
+  eexists.
+  split; try apply H_BINV_fx_v'.
+  intros v0 H_AINV_x_v0 st0.
+  destruct (H_body x v0 H_AINV_x_v0 st0) as [v'' [f'' [st'' [eval_body' H_BINV_fx_v'']]]].
+  eexists.
+  exists body.
+  exists st''.
+  exists v''.
+  split; try reflexivity.
+  split; try apply H_BINV_fx_v''.
+  exists f''.
+  unfold evaluate.
+  assumption.
+  Unshelve.
+  constructor.
+Qed.
+
+(* Theorem EVAL_ELetrec_Fun {A B : Type} (env : sem_env val) (AINV : A -> val -> Prop) (BINV : B -> val -> Prop) (f : A -> B) (fname var : varN) (body : exp) : *)
+(*   (forall (x : A) (v : val), AINV x v -> EVAL (bind_variable_name var v env) body (BINV (f x))) -> *)
+(*   EVAL env (ELetrec [(fname,var,body)] (EVar (Short fname))) ((FUNC AINV BINV) f). *)
+(* Proof. *)
+(*   unfold EVAL, evaluate. *)
+(*   (* intros A B AINV BINV f fname env n var body Henv_update st. *) *)
+(*   intros H_bound st. *)
+(*   do 3 eexists. *)
+(*   simp eval_or_match; simpl. *)
+(*   split. *)
+(*   -  unfold nsLookup. simpl. *)
+(*      rewrite String.eqb_refl. *)
+(*      reflexivity. *)
+(*   - unfold FUNC. *)
+(*     intros x v H. *)
+(*     unfold app_returns. *)
+(*     destruct H as [Hneqx HAINVv]; subst. *)
+(*     destruct (Henv_update v HAINVv st) as [v0 [f0 [st0 [Hevalbody HBINVv0]]]]. *)
+(*     exists v0. *)
+(*     split; try assumption. *)
+(*     unfold app_returns. *)
+(*     intros v1 [Hxeqx HAINVv1] st0'. *)
+(*     destruct (Henv_update v1 HAINVv1 st0') as [v' [f' [st' [Hevalbody' HBINVv1]]]]. *)
+(*     do 4 eexists. *)
+(*     split. *)
+(*     simpl. *)
+(*     rewrite String.eqb_refl. *)
+(*     reflexivity. *)
+(*     split; try assumption. *)
+(*     unfold eval_rel. *)
+(*     unfold bind_variable_name in Hevalbody'. *)
+(*     unfold update_sev in *; simpl in *. *)
+(*     eexists. *)
+(*     unfold evaluate. *)
+(*     apply Hevalbody'. *)
+(*     assumption. *)
+(*     Unshelve. *)
+(*     constructor. *)
+
+
+Lemma string_in_In : forall s l, string_in s l = true <-> In s l.
+Proof.
+  intros s l. split; revert s; induction l.
+  - intros s H. inv H.
+  - intros.
+    unfold string_in in H. break_match.
+    constructor.
+    apply String.eqb_eq.
+    rewrite String.eqb_sym.
+    assumption.
+    right.
+    apply IHl.
+    apply H.
+  - intros s H. inv H.
+  - intros s H.
+    unfold In in H.
+    simpl.
+    break_match; try reflexivity.
+    inv H. rewrite String.eqb_refl in Heqb; inv Heqb.
+    apply IHl. assumption.
+Qed.
+
+Lemma nodup_str_NoDup : forall (l : list string), nodup_str l = true <-> NoDup l.
+Proof.
+  split; induction l; intros.
+  - constructor.
+  - unfold nodup_str in H.
+    break_match. inv H.
+    constructor.
+    intro contra.
+    rewrite <- string_in_In in contra.
+    rewrite contra in Heqb. inv Heqb.
+    apply IHl.
+    assumption.
+  - reflexivity.
+  - inv H.
+    apply IHl in H3.
+    simpl.
+    break_match.
+    rewrite string_in_In in Heqb. contradiction.
+    assumption.
+Qed.
+
+Theorem EVAL_ELetrec_general : forall funs env exp P,
+  NoDup (map (fun '(x,y,z) => x) funs) ->
+  EVAL (update_sev env (build_rec_env funs env (sev env))) exp P ->
+  EVAL env (ELetrec funs exp) P.
+Proof.
+  unfold EVAL, evaluate.
+  intros funs env exp P HNoDup Hexp st.
+  specialize (Hexp st).
+  destruct Hexp as [v [f [st' [Hexp Hinv]]]].
+  exists v. exists f. exists st'.
+  split; try assumption.
+  rewrite <- nodup_str_NoDup in HNoDup.
+  simp eval_or_match in *.
+  rewrite HNoDup.
+  assumption.
+Qed.
+
+(* EQ restricts an invariant to talk about a specific term *)
+Definition EQ {A : Type} (AINV : A -> val -> Prop) (a : A) := fun a' v => (a = a') /\ AINV a' v.
+
+Theorem EVAL_EQ {A : Type} : forall (AINV : A -> val -> Prop) (a : A) (e : exp) (env : sem_env val),
+  EVAL env e (AINV a) -> EVAL env e ((EQ AINV a) a).
+Proof.
+  unfold EVAL.
+  unfold EQ.
+  intros AINV a e env H st.
+  specialize (H st).
+  destruct H as [v [f [st' [Heval Hinv]]]].
+  exists v. exists f. exists st'.
+  auto.
+Qed.
+
+Theorem exists_EQ_INV_iff_INV : forall (A : Type) (AINV : A -> val -> Prop) a v, (exists a', EQ AINV a' a v) <-> AINV a v.
+Proof.
+  unfold EQ.
+  intros A AINV a v.
+  split; intro H.
+  destruct H as [a' [Ha'eqa HAINVa]].
+  auto.
+  exists a.
+  split; auto.
+Qed.
+
 Theorem EVAL_EApp_Opapp {A B : Type} (env : sem_env val) (AINV : A -> val -> Prop) (BINV : B -> val -> Prop)
   (f : A -> B) (a : A) (cl v : exp) :
   EVAL env cl (FUNC AINV BINV f) ->
@@ -188,9 +273,9 @@ Proof.
   unfold eval_rel in Heval_rel.
   destruct Heval_rel as [fuel'' Hevaluate].
   exists v_final.
-  apply (use_maximum_fuel [fuel; fuel'; fuel'']) in Heval_cl.
-  apply (use_maximum_fuel [fuel; fuel'; fuel'']) in Hevaluate.
-  apply (use_maximum_fuel [fuel; fuel'; fuel'']) in Heval_v.
+  apply (use_maximum_fuel _ [fuel; fuel'; fuel'']) in Heval_cl.
+  apply (use_maximum_fuel _ [fuel; fuel'; fuel'']) in Hevaluate.
+  apply (use_maximum_fuel _ [fuel; fuel'; fuel'']) in Heval_v.
   remember (list_max [fuel; fuel'; fuel'']) as the_fuel.
   exists (S the_fuel).
   exists st_final.
@@ -264,7 +349,8 @@ Proof.
   break_match.
   rewrite Hfindfname.
   reflexivity.
-  contradiction.
+  rewrite <- nodup_str_NoDup in HNoDup.
+  rewrite HNoDup in Heqb. inv Heqb.
   unfold eval_rel.
   split.
   eexists.
@@ -275,17 +361,17 @@ Proof.
   assumption.
 Qed.
 
-Theorem Eval_EVar_Recclosure : forall (A B : Type) (AINV : A -> val -> Prop) (BINV : B -> val -> Prop)
+Theorem EVAL_EVar_Recclosure : forall (A B : Type) (AINV : A -> val -> Prop) (BINV : B -> val -> Prop)
                             f fname name body n env cl_env,
+    nsLookup ident_string_beq (Short fname) (sev env) = Some (Recclosure cl_env [(fname,name,body)] fname) ->
    (forall v, AINV n v ->
          EVAL (bind_variable_name name v
                  (update_sev cl_env (build_rec_env [(fname,name,body)] cl_env (sev cl_env))))
               body (BINV (f n))) ->
-    nsLookup ident_string_beq (Short fname) (sev env) = Some (Recclosure cl_env [(fname,name,body)] fname) ->
     EVAL env (EVar (Short fname)) ((FUNC (EQ AINV n) BINV) f).
 Proof.
   unfold EVAL, evaluate.
-  intros A B AINV BINV f fname name body n env cl_env Hbody Hlookup st.
+  intros A B AINV BINV f fname name body n env cl_env Hlookup Hbody st.
   do 3 eexists.
   split.
   - simp eval_or_match; simpl.
@@ -304,9 +390,8 @@ Proof.
     do 4 eexists.
     split; try reflexivity.
     simpl.
-    destruct string_dec.
+    rewrite String.eqb_refl.
     reflexivity.
-    contradiction.
     unfold eval_rel.
     split.
     eexists.
@@ -318,6 +403,48 @@ Proof.
     Unshelve.
     constructor.
 Qed.
+
+(* Theorem EVAL_EVar_Recclosure_noEQ : forall (A B : Type) (AINV : A -> val -> Prop) (BINV : B -> val -> Prop) *)
+(*                             f n v fname name body env cl_env, *)
+(*    AINV n v -> *)
+(*    EVAL (bind_variable_name name v *)
+(*            (update_sev cl_env (build_rec_env [(fname,name,body)] cl_env (sev cl_env)))) *)
+(*      body (BINV (f n)) -> *)
+(*     nsLookup ident_string_beq (Short fname) (sev env) = Some (Recclosure cl_env [(fname,name,body)] fname) -> *)
+(*     EVAL env (EVar (Short fname)) ((FUNC AINV BINV) f). *)
+(* Proof. *)
+(*   unfold EVAL, evaluate. *)
+(*   intros A B AINV BINV f n v fname name body env cl_env HAINV Hbody Hlookup st. *)
+(*   do 3 eexists. *)
+(*   split. *)
+(*   - simp eval_or_match; simpl. *)
+(*     rewrite Hlookup; simpl. *)
+(*     reflexivity. *)
+(*   - unfold FUNC. *)
+(*     intros x v0 HAINVxv. *)
+(*     subst. *)
+(*     destruct (Hbody st) as [v' [f' [st' [Hbody' HBINVfxv']]]]. *)
+(*     exists v'. *)
+(*     split; try assumption. *)
+(*     unfold app_returns. *)
+(*     (* intros v0 HAINVxv0 st0. *) *)
+(*     destruct (Hbody st0) as [v0' [f0' [st0' [Hbody0' HBINVfxv0']]]]. *)
+(*     do 4 eexists. *)
+(*     split; try reflexivity. *)
+(*     simpl. *)
+(*     rewrite String.eqb_refl. *)
+(*     reflexivity. *)
+(*     unfold eval_rel. *)
+(*     split. *)
+(*     eexists. *)
+(*     unfold evaluate. *)
+(*     unfold bind_variable_name, update_sev in *; simpl in *. *)
+(*     rewrite Hbody0'. *)
+(*     reflexivity. *)
+(*     assumption. *)
+(*     Unshelve. *)
+(*     constructor. *)
+(* Qed. *)
 
 Theorem EVAL_ELetrec :
   forall (A B : Type) (AINV : A -> val -> Prop) (BINV : B -> val -> Prop) f fname env n var body,
@@ -332,17 +459,9 @@ Proof.
   do 3 eexists.
   simp eval_or_match; simpl.
   split.
-  - break_match.
-    + unfold nsLookup.
-      simpl.
-      rewrite eqb_refl; simpl.
-      reflexivity.
-    + assert (NoDup [fname]).
-      constructor.
-      intro contra.
-      contradiction.
-      constructor.
-      contradiction.
+  -  unfold nsLookup. simpl.
+     rewrite String.eqb_refl.
+     reflexivity.
   - unfold FUNC, EQ.
     intros x v H.
     destruct H as [Hneqx HAINVv]; subst.
@@ -355,13 +474,55 @@ Proof.
     do 4 eexists.
     split.
     simpl.
-    destruct (string_dec fname fname); try reflexivity; try contradiction.
-    unfold eval_rel.
+    rewrite String.eqb_refl.
+    reflexivity.
     split; try assumption.
-    eexists.
-    unfold evaluate.
+    unfold eval_rel.
     unfold bind_variable_name in Hevalbody'.
     unfold update_sev in *; simpl in *.
+    eexists.
+    unfold evaluate.
+    apply Hevalbody'.
+    assumption.
+    Unshelve.
+    constructor.
+Qed.
+
+Theorem EVAL_ELetrec_noEQ :
+  forall (A B : Type) (AINV : A -> val -> Prop) (BINV : B -> val -> Prop) f fname env var body,
+    (forall n v, AINV n v ->
+          EVAL (bind_variable_name var v
+                  (update_sev env (build_rec_env [(fname,var,body)] env (sev env))))
+            body (BINV (f n))) ->
+    EVAL env (ELetrec [(fname,var,body)] (EVar (Short fname))) ((FUNC AINV BINV) f).
+Proof.
+  unfold EVAL, evaluate.
+  intros A B AINV BINV f fname env var body Henv_update st.
+  do 3 eexists.
+  simp eval_or_match; simpl.
+  split.
+  -  unfold nsLookup. simpl.
+     rewrite String.eqb_refl.
+     reflexivity.
+  - unfold FUNC.
+    intros x v H.
+    destruct (Henv_update x v H st) as [v0 [f0 [st0 [Hevalbody HBINVv0]]]].
+    exists v0.
+    split; try assumption.
+    unfold app_returns.
+    intros v1  HAINVv1 st0'.
+    destruct (Henv_update x v1 HAINVv1 st0') as [v' [f' [st' [Hevalbody' HBINVv1]]]].
+    do 4 eexists.
+    split.
+    simpl.
+    rewrite String.eqb_refl.
+    reflexivity.
+    split; try assumption.
+    unfold eval_rel.
+    unfold bind_variable_name in Hevalbody'.
+    unfold update_sev in *; simpl in *.
+    eexists.
+    unfold evaluate.
     apply Hevalbody'.
     assumption.
     Unshelve.
@@ -369,7 +530,6 @@ Proof.
 Qed.
 
 (* Utilities for Coq provided types or general logic *)
-
 Lemma forall_push_conj : forall (A : Type) (P : Prop) (Q : A -> Prop), inhabited A -> P /\ (forall x, Q x) <->  forall (x : A), P /\ Q x.
 Proof.
   intros.
@@ -479,8 +639,8 @@ Proof.
   split.
   - assumption.
   - intros. destruct (H0 x st) as [v' [fuel' [st'' [Heval' Hother]]]].
-    apply (use_maximum_fuel [fuel; fuel']) in Heval.
-    apply (use_maximum_fuel [fuel; fuel']) in Heval'.
+    apply (use_maximum_fuel _ [fuel; fuel']) in Heval.
+    apply (use_maximum_fuel _ [fuel; fuel']) in Heval'.
     Opaque list_max.
     rewrite Heval in Heval'.
     inv Heval'.
@@ -519,6 +679,7 @@ Qed.
 Lemma EVAL_Forall_eval_or_match_has_value : forall ps env st,
     Forall (fun '(P, x) => EVAL env x P) ps ->
     exists vs st' f, eval_or_match true (rev (map snd ps)) f st env uu uu = (st', Rval vs).
+Proof.
   intros ps0 env1 st1 Hassert.
   generalize dependent st1.
   induction ps0; intro st1.
@@ -611,7 +772,7 @@ Proof.
 Qed.
 
 Theorem EVAL_ECon :
-  forall (Q : val -> Prop) es (ps : list ((val -> Prop) * exp)) stmp name env,
+  forall (Q : val -> Prop) (es : list exp) (ps : list ((val -> Prop) * exp)) stmp name env,
     (map snd ps) = es ->
     nsLookup ident_string_beq name (sec env) = Some (length ps, stmp) ->
     Forall (fun '(P,x) => EVAL env x P) ps ->
@@ -656,4 +817,193 @@ Proof.
   - subst. unfold evaluate in *. rewrite Hevalval in Hevalvals; inv Hevalvals; assumption.
   - apply (more_fuel_same_value f'' f') in Hevalvals; try lia; unfold evaluate in *;
       rewrite Hevalval in Hevalvals; inv Hevalvals; assumption.
+Qed.
+
+Theorem EVAL_ELet_wrong : forall (A B : Type) name e1 e2 env (y : A) (z : B) a_inv b_inv,
+    EVAL env e1 (a_inv y) ->
+    (forall v, a_inv y v -> EVAL (extend_dec_env (Build_sem_env (nsBind name v nsEmpty) nsEmpty) env) e2 (b_inv z)) ->
+    EVAL env (ELet (Some name) e1 e2) (b_inv (let x := y in z)).
+Proof.
+  intros.
+  unfold EVAL in *.
+  intros. unfold evaluate in *.
+  specialize (H st).
+  destruct H as [v [f [st' [He1 H_ainv_y_v]]]].
+  specialize (H0 v H_ainv_y_v st').
+  destruct H0 as [v' [f' [st'' [He2 H_binv_z_v']]]].
+  exists v'. exists (list_max [f; f']). exists st''.
+  split.
+  apply use_maximum_fuel with (fuels := [f; f']) in He1.
+  simp eval_or_match; simpl.
+  rewrite He1; simpl.
+  unfold extend_dec_env, update_sev, nsBind in *; simpl in *.
+  apply use_maximum_fuel with (fuels := [f; f']) in He2.
+  assumption.
+  Transparent list_max.
+  unfold list_max. simpl.
+  lia.
+  unfold list_max. simpl.
+  Opaque list_max.
+  lia.
+  assumption.
+Qed.
+
+Theorem EVAL_ELet : forall (A B : Type) name e1 e2 env (y : A) (f : A -> B) AINV BINV orig,
+    orig = (let x := y in (f x)) ->
+    EVAL env e1 (AINV y) ->
+    (forall v, AINV y v -> EVAL (extend_dec_env (Build_sem_env (nsBind name v nsEmpty) nsEmpty) env) e2 (BINV (f y))) ->
+    EVAL env (ELet (Some name) e1 e2) (BINV orig).
+Proof.
+  intros.
+  unfold EVAL in *.
+  intros. unfold evaluate in *.
+  specialize (H0 st).
+  destruct H0 as [v [f1 [st' [He1 H_ainv_y_v]]]].
+  specialize (H1 v H_ainv_y_v st').
+  destruct H1 as [v' [f2 [st'' [He2 H_binv_z_v']]]].
+  exists v'. exists (list_max [f1; f2]). exists st''.
+  split.
+  apply use_maximum_fuel with (fuels := [f1; f2]) in He1.
+  simp eval_or_match; simpl.
+  rewrite He1; simpl.
+  unfold extend_dec_env, update_sev, nsBind in *; simpl in *.
+  apply use_maximum_fuel with (fuels := [f1; f2]) in He2.
+  assumption.
+  Transparent list_max.
+  unfold list_max. simpl.
+  lia.
+  unfold list_max. simpl.
+  lia.
+  Opaque list_max.
+  rewrite H.
+  assumption.
+Qed.
+
+Definition DECL (st : state ST) (env : sem_env val) (decs : list dec) (st' : state ST) (env' : sem_env val) : Prop :=   exists f,  evaluate_decs f st env decs = (st', Rval env').
+
+Theorem DECL_nil : forall st env, DECL st env [] st empty_sem_env.
+Proof.
+  intros.
+  exists 0.
+  simp evaluate_decs.
+  reflexivity.
+Qed.
+
+Theorem DECL_Dlet : forall (AINV : val -> Prop) st env locs name e,
+    EVAL env e AINV ->
+    exists v st', DECL st env [Dlet locs (Pvar name) e] st' {| sec := nsEmpty; sev := alist_to_ns [(name, v)] |}.
+Proof.
+  unfold EVAL, DECL.
+  intros.
+  destruct (H st) as [v [f [ste [Heval HAINVv]]]].
+  exists v, ste, f.
+  simp evaluate_decs.
+  simpl.
+  unfold evaluate in Heval.
+  rewrite Heval.
+  simp pmatch.
+  simpl.
+  reflexivity.
+Qed.
+
+Theorem DECL_Dletrec : forall env fname varname body st locs,
+    DECL st env [Dletrec locs [(fname,varname,body)]] st
+         {| sec := nsEmpty; sev := alist_to_ns [(fname, (Recclosure env [(fname,varname,body)] fname))] |}.
+Proof.
+  unfold EVAL, DECL.
+  intros.
+  exists 0.
+  simp evaluate_decs; simpl.
+  unfold build_rec_env, nsBind.
+  reflexivity.
+Qed.
+
+Theorem DECL_Dtype : forall tyvars tyname constrs st env locs,
+  NoDup (map fst constrs) ->
+  DECL st env [Dtype locs [(tyvars, tyname, constrs)]] (state_update_next_type_stamp st (next_type_stamp st + 1))
+                {| sec := build_tdefs (next_type_stamp st) [(tyvars, tyname, constrs)] ; sev := nsEmpty |}.
+Proof.
+  unfold DECL.
+  intros.
+  exists 0.
+  simp evaluate_decs; simpl.
+  break_match.
+  - reflexivity.
+  - rewrite <- nodup_str_NoDup in H.
+    assert (forall (l : list (tvarN * list ast_t)),
+    nodup_str (map fst l) =
+      nodup_str (map (fun '(n, _) => n) l)) by
+      ( induction l; try reflexivity;
+        try (break_match; try reflexivity)).
+    specialize (H0 constrs).
+    rewrite H0 in H.
+    rewrite H in Heqb.
+    simpl in Heqb. inv Heqb.
+Qed.
+
+Theorem DECL_cons : forall st env d ds st' st'' env' env'',
+    DECL st env [d] st' env' ->
+    DECL st' (extend_dec_env env' env) ds st'' env'' ->
+    DECL st env (d::ds) st'' (extend_dec_env env'' env').
+Proof.
+  unfold DECL.
+  intros.
+  destruct H.
+  destruct H0.
+  destruct (Compare_dec.lt_eq_lt_dec x x0) as [[f_1_lt_0 | f_1_eq_0] | f_1_gt_0]; eexists.
+  - apply (evaluate_decs_more_fuel_same_value x x0) in H; try lia.
+    rewrite evaluate_decs_cons.
+    rewrite H.
+    rewrite H0.
+    unfold combine_dec_result.
+    reflexivity.
+  - subst.
+    rewrite evaluate_decs_cons.
+    rewrite H.
+    rewrite H0.
+    unfold combine_dec_result.
+    reflexivity.
+  - apply (evaluate_decs_more_fuel_same_value x0 x) in H0; try lia.
+    rewrite evaluate_decs_cons.
+    rewrite H.
+    rewrite H0.
+    unfold combine_dec_result.
+    reflexivity.
+Qed.
+
+(* good_cons_env used when defining new EVAL_EMat for types *)
+
+Definition good_cons_env (pes : list (pat * exp)) (env : sem_env val) (consty : stamp):=
+  Forall (fun '(p,e) => exists con_name ps ty,
+              p = Pcon (Some con_name) ps /\
+                NoDup (pat_bindings p []) /\
+                nsLookup ident_string_beq con_name (sec env) = Some (length ps, TypeStamp (id_to_n con_name) ty) /\
+                stamp_same_type (TypeStamp (id_to_n con_name) ty) consty = true) pes.
+
+(* useful when a recursive function has already been certified and just looking it up *)
+(* one thing to notice is that the recursive environment must be the same as the environment
+ the certificate theorem was proven under. Meaning that reusing that proof in a new context
+ is impossible without environment lemmas *)
+Theorem EVAL_ELetrec_EVAL_EVar : forall A env' env name var body (AINV : A -> val -> Prop) (f : A),
+    EVAL env (ELetrec [(name, var, body)] (EVar (Short name))) (AINV f) ->
+    nsLookup ident_string_beq (Short name) (sev env') =
+      Some (Recclosure env [(name, var, body)] name) ->
+    EVAL env' (EVar (Short name)) (AINV f).
+Proof.
+  intros.
+  intros st.
+  specialize (H st).
+  destruct H as [v [f0 [st' [HELetrec HAINVv]]]].
+  eexists. exists 0. exists st'.
+  split.
+  2: { apply HAINVv. }
+  unfold evaluate in *.
+  simp eval_or_match in *.
+  break_match; try inv HELetrec.
+  simp eval_or_match in *; simpl in *.
+  unfold nsLookup in *; simpl in *.
+  rewrite String.eqb_refl in *; simpl in *.
+  inv HELetrec; clear HELetrec; simpl in *.
+  rewrite H0; simpl.
+  reflexivity.
 Qed.
