theories/MapExample.v
@@ -1,0 +1,229 @@
+Require Export Loader. (* I'd like this to be Coq2CakeML *)
+
+Require Import CakeSem.Namespace.
+Require Import CakeSem.CakeAST.
+Require Import CakeSem.SemanticsAux.
+Require Import CakeSem.Evaluate.
+Require Import CakeSem.EvaluateTheory.
+
+Require Import StructTact.StructTactics.
+Require Import Lists.List.
+Import ListNotations.
+Require Import Lia.
+Require Import Strings.String.
+Open Scope string_scope.
+
+Require Import ExampleInv.
+
+GenerateInvariantAndUpdate list.
+GenerateMatchLemma list.
+  intros.
+  destruct matched;
+    unfold EVAL in *; unfold evaluate in *.
+  - intros.
+    specialize (H2 st).
+    destruct H2 as [v [f [st' [H2 H2']]]].
+    clear H4.
+    inv H2'.
+    simp eval_or_match in H3.
+    assert (@nil PARAM0 = []) by reflexivity.
+    specialize (H3 H st').
+    destruct H3 as [v [f0 [st'0 [H3 H3']]]].
+    clear H.
+    exists v.
+    exists (list_max [f;f0]).
+    exists st'0.
+    simp eval_or_match; simpl.
+    apply (use_maximum_fuel _ [f;f0] _) in H2; simpl in H2.
+    rewrite H2. simpl.
+    simp eval_or_match; simpl.
+    simp pmatch; simpl.
+    unfold good_cons_env in H0.
+    inv H0.
+    destruct H5 as [con_name [ps [ty [H51 [H52 [H53 H54]]]]]].
+    inv H51.
+    rewrite H53.
+    simpl in H54.
+    rewrite PeanoNat.Nat.eqb_eq in H54.
+    subst.
+    simpl.
+    apply (use_maximum_fuel _ [f;f0] _) in H3; simpl in H3; unfold list_max in H3.
+    split.
+    rewrite <- sem_env_id.
+    unfold extend_dec_env in H3; simpl in H3.
+    rewrite <- sem_env_id in H3.
+    apply H3.
+    assumption.
+    unfold list_max; simpl; lia.
+    unfold list_max; simpl; lia.
+  - unfold evaluate in *. intros.
+    specialize (H2 st).
+    destruct H2 as [v [f [st' [H2 H2']]]].
+    clear H3.
+    inv H2'.
+    simp eval_or_match in H4.
+    assert (p::matched = p::matched) by reflexivity.
+    destruct H3 as [v1 [H31 [H32 H33]]].
+    specialize (H4 p matched x v1 H H32 H33 st').
+    clear H.
+    destruct H4 as [v' [f0 [st'0 [H4 H4']]]].
+    exists v'.
+    exists (list_max [f;f0]).
+    exists st'0.
+    simp eval_or_match; simpl.
+    apply (use_maximum_fuel _ [f;f0] _) in H2; simpl in H2; try (simpl;lia).
+    rewrite H2. simpl.
+    simp eval_or_match; simpl.
+    unfold good_cons_env in H0.
+    inv H0; clear H0.
+    simp pmatch; simpl.
+    inv H6.
+    clear H6 H7.
+    destruct H3 as [con_name [ps [ty [H3' [H3_nodup [H3_lookup H3_stamp]]]]]].
+    destruct H5 as [con_name' [ps' [ty' [H5' [H5_nodup [H5_lookup H5_stamp]]]]]].
+    inv H3'. inv H5'.
+    rewrite H5_lookup.
+    simpl.
+    simpl in H5_stamp.
+    rewrite PeanoNat.Nat.eqb_eq in H5_stamp. rewrite H5_stamp; simpl.
+    destruct (string_eq_dec pat_str1 pat_str0).
+    subst.
+    inv H1.
+    assert (In pat_str0 [pat_str0]) by (constructor; reflexivity).
+    contradiction.
+    rewrite <- String.eqb_neq in n.
+    rewrite n; simpl.
+    rewrite H3_lookup; simpl.
+    inv H3_stamp.
+    rewrite PeanoNat.Nat.eqb_eq in H0.
+    subst. simpl.
+    simp pmatch; simpl.
+    split.
+    unfold nsBind, extend_dec_env in H4; simpl in H4.
+    apply more_fuel_same_value with f0.
+    lia.
+    apply H4.
+    assumption.
+Qed.
+
+(* Definition dumb (A : Type) := [id A; id A]. *)
+(* GenerateCertificate dumb. *)
+
+Theorem EVAL_ECon_list_nil :
+  forall A A_INV env,
+    nsLookup ident_string_beq (Short "Nil") (sec env) = Some (0, TypeStamp "Nil" 0) ->
+    EVAL env (ECon (Some (Short "Nil")) []) (list_INV A A_INV []).
+Proof.
+  intros A AINV env HnsLookup st.
+  unfold evaluate.
+  do 3 eexists.
+  split.
+  simp eval_or_match; simpl.
+  rewrite HnsLookup; simpl.
+  simp eval_or_match.
+  unfold build_conv.
+  unfold ident_string_beq in HnsLookup.
+  rewrite HnsLookup. simpl. reflexivity.
+  reflexivity.
+  Unshelve.
+  constructor.
+Qed.
+
+Theorem EVAL_ECon_list_Cons :
+  forall A A_INV env a xs e1 e2,
+    nsLookup ident_string_beq (Short "Cons") (sec env) = Some (2, TypeStamp "Cons" 0) ->
+    EVAL env e1 (A_INV a) ->
+    EVAL env e2 (list_INV A A_INV xs) ->
+    EVAL env (ECon (Some (Short "Cons")) [e1;e2]) (list_INV A A_INV (a::xs)).
+Proof.
+  intros A AINV env a xs e1 e2 HnsLookup He1 He2.
+  unfold EVAL, evaluate in *.
+  intro st.
+  specialize He2 with st.
+  destruct He2 as [v2  [f2  [st2  [Hevale2 HINVe2]]]].
+  specialize He1 with st2.
+  destruct He1 as [v1  [f1  [st1  [Hevale1 HINVe1]]]].
+  apply (more_fuel_same_value f1 (f1 + f2)) in Hevale1.
+  apply (more_fuel_same_value f2 (f1 + f2)) in Hevale2.
+  unfold evaluate in *.
+  (* eexists. *)
+  (* exists (f1 + f2). *)
+  (* eexists. *)
+  do 3 eexists.
+  split.
+  simp eval_or_match; simpl.
+  rewrite HnsLookup; simpl.
+  simp eval_or_match; simpl.
+  rewrite Hevale2; simpl.
+  rewrite Hevale1; simpl.
+  unfold ident_string_beq in HnsLookup.
+  rewrite HnsLookup; simpl.
+  reflexivity.
+  simpl.
+  do 2 eexists.
+  split.
+  reflexivity.
+  split; assumption.
+  lia.
+  lia.
+Qed.
+
+Require Import CakeSem.Evaluate.
+GenerateCertificate map.
+Obligations.
+  intros A AINV B BINV.
+  apply EVAL_EFun.
+  intros f v H.
+  apply EVAL_remove_EQ.
+  - constructor. constructor.
+  - intros x.
+    apply EVAL_ELetrec.
+    induction x.
+    * intros u H'.
+      apply EVAL_EMat_list with A AINV [] (fun a l => (f a)::(map f l)) [].
+      + reflexivity.
+      + good_cons_env_solve.
+      + NoDup_solve.
+      + apply EVAL_EVar with u; try reflexivity; try assumption.
+      + intro.
+        eapply EVAL_ECon_list_nil.
+        reflexivity.
+      + intros aa ab ac ad contra.
+        inv contra.
+    * intros u H'.
+      apply EVAL_EMat_list with A AINV [] (fun a l => (f a)::(map f l)) (a::x).
+      + reflexivity.
+      + good_cons_env_solve.
+      + NoDup_solve.
+      + eapply EVAL_EVar; try reflexivity; try assumption.
+      + intro contra. inv contra.
+      + intros.
+        eapply EVAL_ECon_list_Cons.
+        -- reflexivity.
+        -- eapply EVAL_EApp_Opapp.
+           ** apply EVAL_EVar with v;try reflexivity; try assumption.
+              apply H.
+           ** eapply EVAL_EVar ; try reflexivity; try assumption.
+        -- eapply EVAL_EApp_Opapp.
+           ** eapply EVAL_EVar_Recclosure.
+              ++ intros.
+                 reflexivity.
+              ++ apply IHx.
+           ** eapply EVAL_EVar; try reflexivity; try assumption.
+              unfold EQ. split; inv H0; try reflexivity; try assumption.
+Qed.
+
+FinishProgram "map".
+Obligations.
+  unfold DECL.
+  eexists.
+  simpl.
+  simp evaluate_decs; simpl.
+  simp evaluate_decs; simpl.
+  simp eval_or_match; simpl.
+  reflexivity.
+  Unshelve.
+  constructor.
+Qed.
+
+(* Check cake_prog_map_certificate_thm. *)
